LeanCats/Relations.lean
@@ -1,6 +1,7 @@
 import LeanCats.Data
 
-namespace Event
+namespace CatRel
+open Data
 
 def union (r₁ r₂ : Rel Event Event) := λ x y ↦ r₁ x y ∨ r₂ x y
 def inter (r₁ r₂ : Rel Event Event) := λ x y ↦ r₁ x y ∧ r₂ x y
@@ -13,14 +14,14 @@ instance : Inter (Rel Event Event) := ⟨inter⟩
 @[simp] def fr (rf co : Rel Event Event) (e₁ e₂ : Event) : Prop :=
   ∃w, w.act.op = Op.write ∧ rf w e₁ ∧ co w e₂
 
-@[simp] def R (E : List Event) (e : Event) : Prop :=
-  e ∈ E ∧ e.act.op = Op.read
+@[simp] def R (e : Event) : Prop :=
+  e.act.op = Op.read
 
-@[simp] def W (E : List Event) (e : Event) : Prop :=
-  e ∈ E ∧ e.act.op = Op.write
+@[simp] def W (e : Event) : Prop :=
+  e.act.op = Op.write
 
-@[simp] def M (E : List Event) (e : Event) : Prop :=
-  R E e ∨ W E e
+@[simp] def M (e : Event) : Prop :=
+  R e ∨ W e
 
 @[simp] def Rel.prod (lhs rhs : List Event -> Event -> Prop) (E : List Event) (e₁ e₂ : Event) : Prop :=
   lhs E e₁ ∧ rhs E e₂
@@ -31,4 +32,22 @@ instance : Inter (Rel Event Event) := ⟨inter⟩
 @[simp] def Acyclic (r : Rel Event Event) : Prop
   := Irreflexive (Relation.TransGen r)
 
-end Event
+@[simp] def Rel.internal (evts : Set Event) (e₁ e₂ : Event) : Prop :=
+  e₁.t_id = e₂.t_id ∧ e₁ ∈ evts ∧ e₂ ∈ evts
+
+@[simp] def Rel.external (evts : Set Event) (e₁ e₂ : Event) : Prop :=
+  ¬ (Rel.internal evts e₁ e₂)
+
+@[simp] def Rel.ident (X : CandidateExecution) (e₁ e₂ : Event) : Prop :=
+  e₁ = e₂ -- ∧ e₁ ∈ X.evts
+
+@[simp] def Rel.empty (_ _ : Event) : Prop :=
+  False
+
+@[simp] def Rel.loc (e₁ e₂ : Event) : Prop :=
+  e₁.act.target = e₂.act.target
+
+@[simp] def Rel.ext (e₁ e₂ : Event) : Prop :=
+  e₁.t_id ≠ e₂.t_id
+
+end CatRel
